# 公式推导

------------------

$$
vm = r_1m * \cos{\epsilon_1} \\
cm = \sqrt{(bm)^2 - (am)^2} \\
cm = m\sqrt{b^2 - a^2} \\
cxm = \frac{vm}{bm} * cm \\
cxm = \frac{r_1m * \cos{\epsilon_1}}{bm} * m\sqrt{b^2 - a^2} \\
cxm = \frac{r_1m * \cos{\epsilon_1}}{b} * \sqrt{b^2 - a^2} \\
cx = \frac{r_1 * \cos{\epsilon_1}}{b} * \sqrt{b^2 - a^2} \\
(cx)^2 = \frac{r_1^2 * \cos^2{\epsilon_1}}{b^2} * (b^2 - a^2) \\
$$


$$
cxm = \sqrt{(r_1m)^2 - (am)^2} \\
cxm = m\sqrt{r_1^2 - a^2} \\
cx = \sqrt{r_1^2 - a^2} \\
(cx)^2 = r_1^2 - a^2 \\
$$

$$
\therefore r_1^2 - a^2 = (cx)^2 = \frac{r_1^2 * \cos^2{\epsilon_1}}{b^2} * (b^2 - a^2)\\
r_1^2 - a^2 = \frac{r_1^2(\cos{\epsilon_1})^2}{b^2} * (b^2 - a^2)\\
r_1^2 - a^2 = r_1^2(\cos{\epsilon_1})^2/{b^2} * (b^2 - a^2)\\
r_1^2 = (r_1^2(\cos{\epsilon_1})^2/{b^2} * (b^2 - a^2)) + a^2\\
r_1^2 = a^2 / (1 - \frac{(\cos{\epsilon_1})^2 * (b^2 - a^2)}{b^2})
\\[50px]

r_1^2 * (1 - (\cos{\epsilon_1})^2/{b^2} * (b^2 - a^2)) = a^2\\
1 - (\cos{\epsilon_1})^2/{b^2} * (b^2 - a^2) = \frac{a^2}{r_1^2}\\
(\cos{\epsilon_1})^2/{b^2} * (b^2 - a^2) = 1 - \frac{a^2}{r_1^2}\\
(\cos{\epsilon_1})^2/{b^2} = \frac{1 - \frac{a^2}{r_1^2}}{b^2 - a^2}\\
\begin{cases}
(\cos{\epsilon_1})^2 = \frac{(1 - \frac{a^2}{r_1^2})b^2}{b^2 - a^2}\\
(\cos{\epsilon_2})^2 = \frac{(1 - \frac{a^2}{r_2^2})b^2}{b^2 - a^2}\\
\end{cases}
$$




$$
三角形余角公式：e^2 + d^2 - 2de \times \cos \alpha = n^2 \\
\therefore (r_1m)^2 + (r_2m)^2 - 2r_1r_2m^2 \times \cos(\epsilon_2 - \epsilon_1) = (2R + \Delta_ 1 + \Delta_3)^ 2 \\
(r_2m)^2 = \Delta_p^2 + \Delta_2^2 - 2\Delta_p(\Delta_2 + R) \times \cos (180 - \phi - \alpha)\\
(r_1m)^2 = \Delta_p^2 + \Delta_1^2 - 2\Delta_p(\Delta_1 + R) \times \cos (\phi + \alpha)
$$

