$$
y = kx + b
(x - a)^2 + (y - b)^2 = r^2
$$

$$
G = (1, 1) = (x, y)\\
H = (x_0, y_0)\\
h = y_0 - y\\
i = x_0 - x = H.x - G.x\\
k = tan a = \frac{h}{i}\\
\frac{y_0 - y}{x_0 - x} = k \\
y_0 - y = k(x_0 - x)\\
y = y_0 - k(x_0 - x)
$$

$$
y = y_0 - k(x_0 - x)\\
y = y_0 - kx_0 + kx\\
y = kx - kx_0 + y_0\\
y = kx - (kx_0 - y_0)\\
f(x) = kx + b \\
b = -(kx_0 - y_0)\\
$$

$$
y = kx + b\\
p_1 = (10, 5), p_2 = (3, 8)\\
\begin{cases}
5 = 10k + b\\
8 = 3k + b
\end{cases}
可以得到 k, b\\
从而得到 y = [k]x + [b]
$$

$$
A = (2, 3)\\
B = (3, 5)\\
C = (5, 4)\\
D = (7, 3)\\
$$

$$
\begin{align}
y &= kx + b\\
&\begin{cases}
3 = 2k + b\\
5 = 3k + b\\
4 = 5k + b\\
3 = 7k + b\\
\end{cases}\\
3 &= 2k + b\\
f(x) &= kx + b \\
y &= f(x) \\
f(k, b) &= [3 - (2k + b)]^2 + [5 - (3k + b)]^2 + [4 - (5k + b)]^2 + [3 - (7k + b)]^2

\end{align}
$$


$$
k = h / w\\
k = h / \Delta x\\
h = f(x + \Delta x) - f(x)\\
k = \frac{f(x + \Delta x) - f(x)}{\Delta x}\\
k = \lim_{\Delta x -> 0}\frac{f(x + \Delta x) - f(x)}{\Delta x}\\
f(x + \Delta x) - f(x)\\
= (x + \Delta x)^2 - x^2\\
= x^2 + 2x • \Delta x + \Delta x^2 - x^2\\
= 2x • \Delta x + \Delta x^2\\
= \Delta x(2x + \Delta x)\\[20px]
k = \lim_{\Delta x -> 0}\frac{f(x + \Delta x) - f(x)}{\Delta x}\\
= \lim_{\Delta x -> 0}\frac{\Delta x(2x + \Delta x)}{\Delta x}\\
= \lim_{\Delta x -> 0}2x + \Delta x\\
= 2x
$$

$$
k = 2x\\
p = (2, 4)\\
y = kx + b\\
k = 4\\
4 = 8 + b\\
b = -4\\
y = 4x - 4\\[20px]

k = 2x\\
p = (1, 1)\\
y - kx + b\\
k = 2\\
1 = 2 + b\\
b = -1\\
y = 2x - 1\\[20px]

y = x^2 的导数 = 2x\\
x^2 的导数 = 0 \\
x = 0
$$

$$
\sum_{i = 1}^{4} [y_i - (kx_i + b)]^2\\
\frac{\partial}{\partial x} x^2 = 2x\\
\frac{\partial}{\partial x} \sum_{i = 1}^{n}x_i^2 = 2\sum_{i = 1}^{n}x_i\\
f(k, b) = [3 - (2k + b)]^2 + [5 - (3k + b)]^2 + [4 - (5k + b)]^2 + [3 - (7k + b)]^2\\
$$



$$
y = x^2 = f(x)\\
f(x) 的导数 = 2x \\
\frac{\partial}{\partial x} f = 2x \\
\lim_{\Delta x -> 0}
在函数f中，关于细分 \Delta x 的导数 = 2x \\
\partial x\ 细分 \Delta x\\
\partial y\ 细分 \Delta y\\
\partial p\ 细分 \Delta p\\
\frac{\partial}{\partial x} f = 2x \\
\frac{\partial}{\partial y} f = 2x \\
$$

$$
f(x) = ax^2 + bx + c\\
ax^2 + bx + c = 0\\
x = \frac{±\sqrt{b^2 - 4ac} - b}{2a}\\
x = \frac{-b}{2a}
$$

$$
f(x) = ax^2 + bx + c\\
\frac{f(x + \Delta x) - f(x)}{\Delta x}\\
a(x + \Delta x)^2 + b(x + \Delta x) + c - ax^2 - bx - c\\
a(x^2 + 2x •\Delta x + \Delta x^2) + bx + b\Delta x + c - ax^2 - bx - c\\
ax^2 + 2ax •\Delta x + a\Delta x^2 + bx + b\Delta x + c - ax^2 - bx - c\\
2ax •\Delta x + a\Delta x^2 + b\Delta x\\
\Delta x(2ax + a\Delta x + b)\\
\frac{\Delta x(2ax + a\Delta x + b)}{\Delta x}\\
2ax + a\Delta x + b\\
\lim_{\Delta x -> 0}2ax + a\Delta x + b \\
k = 2ax + b
$$

$$
k = 2ax + o\\
y = kx + b\\
a = 4\\
o = 3\\
c = 10\\
k = 8x + 3\\
x = 1\\
y = 17\\
k = 11\\
17 = 11 + b\\
b = 6\\
y = 11x + 6\\
$$

$$
2ax + o = 0\\
2ax = -o\\
x = \frac{-b}{2a}
$$

$$
\frac{\partial}{\partial x}(x + 6)^2\\
\frac{(x + \Delta x + 6)^2 - (x + 6)^2}{\Delta x}\\
\begin{align}
& (\Delta x + x + 6)^2 - (x + 6)^2\\
= &\Delta x^2 + 2\Delta x(x + 6) + (x + 6)^2 - (x + 6)^2\\
= &\Delta x^2 + 2\Delta x(x + 6)\\
= &\Delta x(\Delta x + 2(x + 6))\\
\end{align} \\
\frac{(x + \Delta x + 6)^2 - (x + 6)^2}{\Delta x} = \Delta x + 2(x + 6)\\
\frac{\partial}{\partial x}(x + 6)^2 = 2(x + 6)
$$

$$
\frac{\partial}{\partial x} (4x + 6)^2\\
\frac{f(\Delta x + x) - f(x)}{\Delta x}\\
\begin{align}
&f(\Delta x + x) - f(x)\\
= &(4(\Delta x + x) + 6)^2 - (4x + 6)^2 \\
= &(16(\Delta x + x)^2 + 2\times24(\Delta x + x) + 6^2) - (4x + 6)^2\\
= &(16(\Delta x + x)^2 + 2\times24(\Delta x + x) + 6^2) - (4x + 6)^2\\
\end{align}
$$





